ulib/experimental/Steel.V.Effect.fst
@@ -1,0 +1,464 @@
+(*
+   Copyright 2020 Microsoft Research
+
+   Licensed under the Apache License, Version 2.0 (the "License");
+   you may not use this file except in compliance with the License.
+   You may obtain a copy of the License at
+
+       http://www.apache.org/licenses/LICENSE-2.0
+
+   Unless required by applicable law or agreed to in writing, software
+   distributed under the License is distributed on an "AS IS" BASIS,
+   WITHOUT WARRANTIES OR CONDITIONS OF ANY KIND, either express or implied.
+   See the License for the specific language governing permissions and
+   limitations under the License.
+*)
+
+module Steel.V.Effect
+
+module Sem = Steel.Semantics.Hoare.MST
+module Mem = Steel.Memory
+open Steel.Semantics.Instantiate
+module FExt = FStar.FunctionalExtensionality
+
+#set-options "--ide_id_info_off"
+
+#set-options "--warn_error -330"  //turn off the experimental feature warning
+
+[@@ __steel_reduce__]
+let req_to_act_req (#pre:pre_t) (req:req_t pre) : Sem.l_pre #state (hp_of pre) =
+  fun m0 -> interp (hp_of pre) m0 /\ (value_is_valid_complete pre m0; req (sel_of pre m0))
+
+unfold
+let to_post (#a:Type) (post:post_t a) = fun x -> (hp_of (post x))
+
+// [@@ __steel_reduce__]
+
+let ens_to_act_ens0 (#pre:pre_t) (#a:Type) (#post:post_t a) (ens:ens_t pre a post)
+  (m0: mem)
+  (x: a)
+  (m1: mem)
+: Tot prop
+=
+    interp (hp_of pre) m0 /\ interp (hp_of (post x)) m1 /\ (value_is_valid_complete pre m0; value_is_valid_complete (post x) m1; ens (sel_of pre m0) x (sel_of (post x) m1))
+
+let ens_to_act_ens (#pre:pre_t) (#a:Type) (#post:post_t a) (ens:ens_t pre a post)
+: Sem.l_post #state #a (hp_of pre) (to_post post)
+= ens_to_act_ens0 ens
+
+unfold
+let ens_to_act_ens1 (#pre:pre_t) (#a:Type) (#post:post_t a) (ens:ens_t pre a post)
+  (m0: mem)
+  (x: a)
+  (m1: mem)
+: Tot prop
+=
+    interp (hp_of pre) m0 /\
+    interp (hp_of (post x)) m1 /\ (
+      (value_is_valid pre (sel_of pre m0) /\
+      value_is_valid (post x) (sel_of (post x) m1)) ==> (
+        ens (sel_of pre m0) x (sel_of (post x) m1)
+    ))
+
+let ens_to_act_ens1_correct
+  (#pre:pre_t) (#a:Type) (#post:post_t a) (ens:ens_t pre a post)
+  (m0: mem)
+  (x: a)
+  (m1: mem)
+: Lemma
+  (requires (ens_to_act_ens1 ens m0 x m1))
+  (ensures (ens_to_act_ens ens m0 x m1))
+= value_is_valid_complete pre m0;
+  value_is_valid_complete (post x) m1
+
+val can_be_split_3_interp (p1 p2 q r:slprop u#1) (m:mem)
+: Lemma
+  (requires p1 `slimp` p2 /\  interp (p1 `Mem.star` q `Mem.star` r) m)
+  (ensures interp (p2 `Mem.star` q `Mem.star` r) m)
+
+let can_be_split_3_interp p1 p2 q r m =
+  Mem.star_associative p1 q r;
+  Mem.star_associative p2 q r;
+  slimp_star p1 p2 (q `Mem.star` r) (q `Mem.star` r)
+
+let repr (a:Type) (_:bool) (pre:pre_t) (post:post_t a) (req:req_t pre) (ens:ens_t pre a post) =
+  Sem.action_t #state #a (hp_of pre) (to_post post)
+    ((req_to_act_req req))
+    ((ens_to_act_ens ens))
+
+let nmst_get (#st:Sem.st) ()
+  : Sem.Mst (Sem.full_mem st)
+           (fun _ -> True)
+           (fun s0 s s1 -> s0 == s /\ s == s1)
+  = NMST.get ()
+
+let return_ a x #p = fun _ ->
+      x
+
+#push-options "--fuel 0 --ifuel 0"
+
+val req_frame (frame:vprop) (snap:valid_value frame) : mprop (hp_of frame)
+
+let req_frame' (frame:vprop) (snap:valid_value frame) (m:mem) : prop =
+  interp (hp_of frame) m /\ sel_of frame m == snap
+
+let req_frame frame snap =
+  req_frame' frame snap
+
+#push-options "--z3rlimit 20 --fuel 1 --ifuel 1 --query_stats" // ifuel 1 necessary because of the Sem record
+
+val frame00 (#a:Type)
+          (#framed:bool)
+          (#pre:pre_t)
+          (#post:post_t a)
+          (#req:req_t pre)
+          (#ens:ens_t pre a post)
+          ($f:repr a framed pre post req ens)
+          (frame:vprop)
+  : repr a
+    true
+    (pre `star` frame)
+    (fun x -> post x `star` frame)
+    (fun h -> req (vselect h pre))
+    (fun h0 r h1 -> req (vselect h0 pre) /\ ens (vselect h0 pre) r (vselect h1 (post r)) /\
+     vselect h0 frame == vselect h1 frame)
+
+#restart-solver
+let frame00 #a #framed #pre #post #req #ens f frame =
+  fun frame' ->
+      let m00 = nmst_get () in
+      let m0 = core_mem m00 in
+      vselect_correct (pre `star` frame) pre m0;
+      vselect_correct (pre `star` frame) frame m0;
+      let snap = Ghost.hide (sel_of frame m0) in
+
+      let x = Sem.run #state #_ #_ #_ #_ #_ frame' (Sem.Frame (Sem.Act f) (hp_of frame) (req_frame frame snap)) in
+
+      let m01 = nmst_get () in
+      let m1 = core_mem m01 in
+      vselect_correct (post x `star` frame) (post x) m1;
+      vselect_correct (post x `star` frame) frame m1;
+
+      x
+
+#pop-options
+
+let bind_ens_intro (#a:Type) (#b:Type)
+  (#pre_f:pre_t) (#post_f:post_t a)
+  (req_f:req_t pre_f) (ens_f:ens_t pre_f a post_f)
+  (#pre_g:a -> pre_t) (#post_g:a -> post_t b)
+  (#pr:a -> prop)
+  (ens_g:(x:a -> ens_t (pre_g x) b (post_g x)))
+  (frame_f:vprop) (frame_g:a -> vprop)
+  (post:post_t b)
+  (p1:squash (can_be_split_forall_dep pr (fun x -> post_f x `star` frame_f) (fun x -> pre_g x `star` frame_g x)))
+  (p2:squash (can_be_split_post (fun x y -> post_g x y `star` frame_g x) post))
+  (m0: valid_value (pre_f `star` frame_f))
+  (y: b)
+  (m2: valid_value (post y))
+  (x: a)
+  (h1: valid_value (post_f x `star` frame_f))
+: Lemma
+  (requires (
+    req_f (vselect m0 pre_f) /\
+    pr x /\
+    vselect m0 frame_f == vselect h1 frame_f /\
+    vselect h1 (frame_g x) == vselect m2 (frame_g x) /\
+    ens_f (vselect m0 pre_f) x (vselect h1 (post_f x)) /\
+    ens_g x (vselect h1 (pre_g x)) y (vselect m2 (post_g x y))
+  ))
+  (ensures (
+    bind_ens req_f ens_f ens_g frame_f frame_g post p1 p2 m0 y m2
+  ))
+= ()
+
+#push-options "--print_implicits --ifuel 1 --fuel 1 --query_stats --z3rlimit_factor 24"
+
+#restart-solver
+let bind a b #framed_f #framed_g #pre_f #post_f #req_f #ens_f #pre_g #post_g #req_g #ens_g #frame_f #frame_g #post #_ #_ #pr #p1 #p2 f g =
+  fun frame ->
+    let m0 = nmst_get () in
+    value_is_valid_complete (pre_f `star` frame_f) (core_mem m0);
+    let v0 = Ghost.hide (sel_of (pre_f `star` frame_f) (core_mem m0)) in
+    let x = frame00 f frame_f frame in
+    let m1 = nmst_get () in
+    value_is_valid_complete (post_f x `star` frame_f) (core_mem m1);
+    let v1 = Ghost.hide (sel_of (post_f x `star` frame_f) (core_mem m1)) in
+    assert (interp (hp_of (post_f x `star` frame_f)) m1);
+    assert (ens_f (vselect v0 pre_f) x (vselect v1 (post_f x)));
+    assert (vselect v0 frame_f == vselect v1 frame_f);
+    assert (pr x);
+    assert ((post_f x `star` frame_f) `can_be_split` (pre_g x `star` frame_g x));
+    assert (req_g x (vselect v1 (pre_g x)));
+    vselect_correct (post_f x `star` frame_f) (pre_g x `star` frame_g x) (core_mem m1);
+    let v1' = Ghost.hide (sel_of (pre_g x `star` frame_g x) (core_mem m1)) in
+    assert (Ghost.reveal v1' == vselect v1 (pre_g x `star` frame_g x));
+    assert (req_g x (vselect v1' (pre_g x)));
+    can_be_split_slimp
+      (post_f x `star` frame_f)
+      (pre_g x `star` frame_g x);
+    can_be_split_3_interp
+      (hp_of (post_f x `star` frame_f))
+      (hp_of (pre_g x `star` frame_g x))
+      frame (locks_invariant Set.empty m1) m1;
+    let y = frame00 (g x) (frame_g x) frame in
+    let m2 = nmst_get () in
+    let prf () : Lemma (
+      ens_to_act_ens1 (bind_ens req_f ens_f ens_g frame_f frame_g post p1 p2) (core_mem m0) y (core_mem m2)
+    ) =
+      value_is_valid_complete (post_g x y `star` frame_g x) (core_mem m2);
+      let v2' = Ghost.hide (sel_of (post_g x y `star` frame_g x) (core_mem m2)) in
+      assert (ens_g x (vselect v1' (pre_g x)) y (vselect v2' (post_g x y))); 
+      assert (vselect v2' (frame_g x) == vselect v1' (frame_g x));
+      assert (vselect v1' (frame_g x) == vselect v1 (frame_g x));
+      vselect_correct (post_g x y `star` frame_g x) (post y) (core_mem m2);
+      vselect_correct (post y) (post_g x y `star` frame_g x) (core_mem m2);
+      let v2 = Ghost.hide (sel_of (post y) (core_mem m2)) in
+      assert (vselect v2 (frame_g x) == vselect v2' (frame_g x));
+      assert (vselect v2 (post_g x y) == vselect v2' (post_g x y));
+      assert (ens_g x (vselect v1 (pre_g x)) y (vselect v2 (post_g x y)));
+      bind_ens_intro req_f ens_f ens_g frame_f frame_g post p1 p2 v0 y v2 x v1
+    in
+    prf ();
+    ens_to_act_ens1_correct (bind_ens req_f ens_f ens_g frame_f frame_g post p1 p2) (core_mem m0) y (core_mem m2);
+    can_be_split_slimp
+      (post_g x y `star` frame_g x)
+      (post y);
+    can_be_split_3_interp
+      (hp_of (post_g x y `star` frame_g x))
+      (hp_of (post y))
+      frame (locks_invariant Set.empty m2) m2;
+    y
+
+#pop-options
+
+(*
+#push-options "--fuel 1 --ifuel 1 --z3rlimit 20"
+
+let subcomp_opaque a #framed_f #framed_g #pre_f #post_f #req_f #ens_f #pre_g #post_g #req_g #ens_g #fr #_ #p1 #p2 f =
+  fun frame ->
+    let m0 = nmst_get () in
+    let h0 = mk_rmem pre_g (core_mem m0) in
+    can_be_split_trans pre_g (pre_f `star` fr) pre_f;
+    can_be_split_trans pre_g (pre_f `star` fr) fr;
+
+    can_be_split_3_interp (hp_of pre_g) (hp_of (pre_f `star` fr)) frame (locks_invariant Set.empty m0) m0;
+
+    focus_replace pre_g (pre_f `star` fr) pre_f (core_mem m0);
+
+    let x = frame00 f fr frame in
+
+    let m1 = nmst_get () in
+    let h1 = mk_rmem (post_g x) (core_mem m1) in
+
+    let h0' = mk_rmem (pre_f `star` fr) (core_mem m0) in
+    let h1' = mk_rmem (post_f x `star` fr) (core_mem m1) in
+    // From frame00
+    assert (frame_opaque fr (focus_rmem h0' fr) (focus_rmem h1' fr));
+    // Replace h0'/h1' by h0/h1
+    focus_replace pre_g (pre_f `star` fr) fr (core_mem m0);
+    focus_replace (post_g x) (post_f x `star` fr) fr (core_mem m1);
+    assert (frame_opaque fr (focus_rmem h0 fr) (focus_rmem h1 fr));
+
+    can_be_split_trans (post_g x) (post_f x `star` fr) (post_f x);
+    can_be_split_trans (post_g x) (post_f x `star` fr) fr;
+
+    can_be_split_3_interp (hp_of (post_f x `star` fr)) (hp_of (post_g x)) frame (locks_invariant Set.empty m1) m1;
+
+    focus_replace (post_g x) (post_f x `star` fr) (post_f x) (core_mem m1);
+
+    x
+
+#pop-options
+
+let lemma_rewrite (p:Type) : Lemma (requires T.rewrite_with_tactic vc_norm p) (ensures p)
+  = T.unfold_rewrite_with_tactic vc_norm p
+
+let lemma_norm_opaque (p:Type) : Lemma (requires norm_opaque p) (ensures p) = ()
+
+(** Need to manually remove the rewrite_with_tactic marker here *)
+let lemma_subcomp_pre_opaque_aux1 (#a:Type)
+  (#pre_f:pre_t) (#post_f:post_t a) (req_f:req_t pre_f) (ens_f:ens_t pre_f a post_f)
+  (#pre_g:pre_t) (#post_g:post_t a) (req_g:req_t pre_g) (ens_g:ens_t pre_g a post_g)
+  (#frame:vprop)
+  (p1:squash (can_be_split pre_g (pre_f `star` frame)))
+  (p2:squash (equiv_forall post_g (fun x -> post_f x `star` frame)))
+  : Lemma
+  (requires subcomp_pre req_f ens_f req_g ens_g p1 p2)
+  (ensures  (can_be_split_trans pre_g (pre_f `star` frame) pre_f;
+    (forall (h0:hmem pre_g). req_g (mk_rmem pre_g h0) ==> req_f (focus_rmem (mk_rmem pre_g h0) pre_f)) /\
+    (forall (h0:hmem pre_g) (x:a) (h1:hmem (post_g x)). (
+
+     can_be_split_trans (post_g x) (post_f x `star` frame) (post_f x);
+     can_be_split_trans (pre_g) (pre_f `star` frame) frame;
+     can_be_split_trans (post_g x) (post_f x `star` frame) frame;
+
+     (req_g (mk_rmem pre_g h0) /\
+      ens_f (focus_rmem (mk_rmem pre_g h0) pre_f) x (focus_rmem (mk_rmem (post_g x) h1) (post_f x)) /\
+      frame_equalities frame
+        (focus_rmem (mk_rmem pre_g h0) frame)
+        (focus_rmem (mk_rmem (post_g x) h1) frame))
+
+        ==> ens_g (mk_rmem pre_g h0) x (mk_rmem (post_g x) h1)
+       ))))
+  = lemma_rewrite (squash (
+      can_be_split_trans pre_g (pre_f `star` frame) pre_f;
+      (forall (h0:hmem pre_g). req_g (mk_rmem pre_g h0) ==> req_f (focus_rmem (mk_rmem pre_g h0) pre_f)) /\
+      (forall (h0:hmem pre_g) (x:a) (h1:hmem (post_g x)). (
+         can_be_split_trans (post_g x) (post_f x `star` frame) (post_f x);
+         can_be_split_trans (pre_g) (pre_f `star` frame) frame;
+         can_be_split_trans (post_g x) (post_f x `star` frame) frame;
+
+         (req_g (mk_rmem pre_g h0) /\
+          ens_f (focus_rmem (mk_rmem pre_g h0) pre_f) x (focus_rmem (mk_rmem (post_g x) h1) (post_f x)) /\
+          frame_equalities frame
+            (focus_rmem (mk_rmem pre_g h0) frame)
+            (focus_rmem (mk_rmem (post_g x) h1) frame))
+
+            ==> ens_g (mk_rmem pre_g h0) x (mk_rmem (post_g x) h1)
+      ))
+    ))
+
+#push-options "--no_tactics"
+
+let lemma_subcomp_pre_opaque_aux2 (#a:Type)
+  (#pre_f:pre_t) (#post_f:post_t a) (req_f:req_t pre_f) (ens_f:ens_t pre_f a post_f)
+  (#pre_g:pre_t) (#post_g:post_t a) (req_g:req_t pre_g) (ens_g:ens_t pre_g a post_g)
+  (#frame:vprop)
+  (p1:squash (can_be_split pre_g (pre_f `star` frame)))
+  (p2:squash (equiv_forall post_g (fun x -> post_f x `star` frame)))
+  : Lemma
+  (requires  (can_be_split_trans pre_g (pre_f `star` frame) pre_f;
+    (forall (h0:hmem pre_g). req_g (mk_rmem pre_g h0) ==> req_f (focus_rmem (mk_rmem pre_g h0) pre_f)) /\
+    (forall (h0:hmem pre_g) (x:a) (h1:hmem (post_g x)). (
+
+     can_be_split_trans (post_g x) (post_f x `star` frame) (post_f x);
+     can_be_split_trans (pre_g) (pre_f `star` frame) frame;
+     can_be_split_trans (post_g x) (post_f x `star` frame) frame;
+
+     (req_g (mk_rmem pre_g h0) /\
+      ens_f (focus_rmem (mk_rmem pre_g h0) pre_f) x (focus_rmem (mk_rmem (post_g x) h1) (post_f x)) /\
+      frame_equalities frame
+        (focus_rmem (mk_rmem pre_g h0) frame)
+        (focus_rmem (mk_rmem (post_g x) h1) frame))
+
+        ==> ens_g (mk_rmem pre_g h0) x (mk_rmem (post_g x) h1)
+       ))))
+
+  (ensures subcomp_pre_opaque req_f ens_f req_g ens_g p1 p2)
+  =  lemma_norm_opaque (squash (
+
+    can_be_split_trans pre_g (pre_f `star` frame) pre_f;
+    (forall (h0:hmem pre_g). req_g (mk_rmem pre_g h0) ==> req_f (focus_rmem (mk_rmem pre_g h0) pre_f)) /\
+    (forall (h0:hmem pre_g) (x:a) (h1:hmem (post_g x)). (
+
+     can_be_split_trans (post_g x) (post_f x `star` frame) (post_f x);
+     can_be_split_trans (pre_g) (pre_f `star` frame) frame;
+     can_be_split_trans (post_g x) (post_f x `star` frame) frame;
+
+     (req_g (mk_rmem pre_g h0) /\
+      ens_f (focus_rmem (mk_rmem pre_g h0) pre_f) x (focus_rmem (mk_rmem (post_g x) h1) (post_f x)) /\
+      frame_opaque frame
+        (focus_rmem (mk_rmem pre_g h0) frame)
+        (focus_rmem (mk_rmem (post_g x) h1) frame))
+
+        ==> ens_g (mk_rmem pre_g h0) x (mk_rmem (post_g x) h1)
+       ))
+  ))
+
+let lemma_subcomp_pre_opaque (#a:Type)
+  (#pre_f:pre_t) (#post_f:post_t a) (req_f:req_t pre_f) (ens_f:ens_t pre_f a post_f)
+  (#pre_g:pre_t) (#post_g:post_t a) (req_g:req_t pre_g) (ens_g:ens_t pre_g a post_g)
+  (#frame:vprop)
+  (p1:squash (can_be_split pre_g (pre_f `star` frame)))
+  (p2:squash (equiv_forall post_g (fun x -> post_f x `star` frame)))
+  : Lemma
+  (requires subcomp_pre req_f ens_f req_g ens_g p1 p2)
+  (ensures subcomp_pre_opaque req_f ens_f req_g ens_g p1 p2)
+  = lemma_subcomp_pre_opaque_aux1 req_f ens_f req_g ens_g p1 p2;
+    lemma_subcomp_pre_opaque_aux2 req_f ens_f req_g ens_g p1 p2
+
+#pop-options
+
+*)
+
+let subcomp a #framed_f #framed_g #pre_f #post_f #req_f #ens_f #pre_g #post_g #req_g #ens_g #fr #_ #p1 #p2 f =
+  admit ()
+
+(*
+  lemma_subcomp_pre_opaque req_f ens_f req_g ens_g p1 p2;
+  subcomp_opaque a #framed_f #framed_g #pre_f #post_f #req_f #ens_f #pre_g #post_g #req_g #ens_g #fr #_ #p1 #p2 f
+*)
+
+#push-options "--z3rlimit_factor 8 --fuel 1 --ifuel 1"
+
+let bind_pure_steel_ a b #wp #pre #post #req #ens f g
+  = FStar.Monotonic.Pure.elim_pure_wp_monotonicity wp;
+    fun frame ->
+      let x = f () in
+      g x frame
+
+#pop-options
+
+(* We need a bind with DIV to implement par, using reification *)
+
+unfold
+let bind_div_steel_req (#a:Type) (wp:pure_wp a)
+  (#pre_g:pre_t) (req_g:a -> req_t pre_g)
+: req_t pre_g
+= FStar.Monotonic.Pure.elim_pure_wp_monotonicity wp;
+  fun h -> wp (fun _ -> True) /\ (forall x. (req_g x) h)
+
+unfold
+let bind_div_steel_ens (#a:Type) (#b:Type)
+  (wp:pure_wp a)
+  (#pre_g:pre_t) (#post_g:post_t b) (ens_g:a -> ens_t pre_g b post_g)
+: ens_t pre_g b post_g
+= fun h0 r h1 -> wp (fun _ -> True) /\ (exists x. ens_g x h0 r h1)
+
+#push-options "--z3rlimit 20 --fuel 2 --ifuel 1"
+let bind_div_steel (a:Type) (b:Type)
+  (wp:pure_wp a)
+  (framed:eqtype_as_type bool)
+  (pre_g:pre_t) (post_g:post_t b) (req_g:a -> req_t pre_g) (ens_g:a -> ens_t pre_g b post_g)
+  (f:eqtype_as_type unit -> DIV a wp) (g:(x:a -> repr b framed pre_g post_g (req_g x) (ens_g x)))
+: repr b framed pre_g post_g
+    (bind_div_steel_req wp req_g)
+    (bind_div_steel_ens wp ens_g)
+= FStar.Monotonic.Pure.elim_pure_wp_monotonicity wp;
+  fun frame ->
+  let x = f () in
+  g x frame
+#pop-options
+
+polymonadic_bind (DIV, SteelBase) |> SteelBase = bind_div_steel
+#pop-options
+
+let par0 (#aL:Type u#a) (#preL:vprop) (#postL:aL -> vprop)
+         (f:repr aL false preL postL (fun _ -> True) (fun _ _ _ -> True))
+         (#aR:Type u#a) (#preR:vprop) (#postR:aR -> vprop)
+         (g:repr aR false preR postR (fun _ -> True) (fun _ _ _ -> True))
+  : SteelT (aL & aR)
+    (preL `star` preR)
+    (fun y -> postL (fst y) `star` postR (snd y))
+  = Steel?.reflect (fun frame -> Sem.run #state #_ #_ #_ #_ #_ frame (Sem.Par (Sem.Act f) (Sem.Act g)))
+
+(*
+ * AR: Steel is not marked reifiable since we intend to run Steel programs natively
+ *     However to implement the par combinator we need to reify a Steel thunk to its repr
+ *     We could implement it better by having support for reification only in the .fst file
+ *     But for now assuming a (Dv) function
+ *)
+assume val reify_steel_comp
+  (#a:Type) (#framed:bool) (#pre:vprop) (#post:a -> vprop) (#req:req_t pre) (#ens:ens_t pre a post)
+  ($f:unit -> SteelBase a framed pre post req ens)
+  : Dv (repr a framed pre post req ens)
+
+let par f g =
+  par0 (reify_steel_comp f) (reify_steel_comp g)
+
+let action_as_repr (#a:Type) (#p:slprop) (#q:a -> slprop) (f:action_except a Set.empty p q)
+  : repr a false (to_vprop p) (fun x -> to_vprop (q x)) (fun _ -> True) (fun _ _ _ -> True)
+  = Steel.Semantics.Instantiate.state_correspondence Set.empty; f
+
+let as_action #a #p #q f = Steel?.reflect (action_as_repr f)
